added support for `epsilon` operator, including notation and tactic

src/util/classical.lean
@@ -1,7 +1,10 @@
 
 import meta.expr
+import util.meta.tactic
 
 universe variables u v
+
+notation `ε` binders `, ` r:(scoped p, classical.epsilon p) := r
 
 namespace classical
 
@@ -11,13 +14,22 @@ variables {p q : α → Prop}
 variables Hpq : ∀ x, p x → q x
 variables Hex : ∃ x, p x
 
-include Hpq
+include Hpq Hex
 
 lemma some_spec'
 : q (some Hex) :=
 begin
   apply Hpq,
   apply some_spec
+end
+
+variable [nonempty α]
+
+lemma epsilon_spec'
+: q (epsilon p) :=
+begin
+  apply Hpq,
+  apply epsilon_spec Hex,
 end
 
 end classical
@@ -37,4 +49,20 @@ do t ← target,
    interactive.intro id,
    try `[intros h, apply h]
 
-run_cmd add_interactive [`apply_some_spec]
+meta def apply_epsilon_spec (ex : parse $ optional texpr)
+  (id : parse $ optional (tk "with" *> ident_)) : tactic unit :=
+focus1 $
+do t ← target,
+   (l,_) ← solve_aux t (do
+     e ← to_expr ``(classical.epsilon _),
+     v ← mk_fresh_name,
+     generalize e v,
+     (expr.pi v bi t e) ← target,
+     return (expr.lam v bi t e)),
+   refine ``(@classical.epsilon_spec' _ _ %%l _ _ _),
+   `[simp only],
+   interactive.intro id,
+   try `[intros h, apply h],
+   all_goals (auto <|> ↑ex >>= tactic.refine <|> return ())
+
+run_cmd add_interactive [`apply_some_spec,`apply_epsilon_spec]
